The new enconding using subtypeOf seems robust.

ref_impl/src/verifier/experiments/fstar_experiments/project2/testing.fst
@@ -6,8 +6,7 @@ open BosqueTypes
 
 (* --------------------------------------------------------------- *)
 
-let aaa = BTuple 2 (SCons (BInt 3) 1 (SCons (BBool true) 0 SNil))
-// let bb = extractTuple 2 aaa
+let test_a = BTuple 2 (SCons (BInt 3) 1 (SCons (BBool true) 0 SNil))
 
 let oktest = BTuple 2 (SCons (BInt 3) 1 (SCons (BBool true) 0 SNil))
 let oktest2 = nthTupleType 10 2 oktest
@@ -19,9 +18,7 @@ let testa1 = subtypeOf (BUnionType BIntType BBoolType) (BNoneType)
 let testa2 = subtypeOf (BUnionType BIntType BBoolType) (BUnionType BNoneType BBoolType)
 let testa3 = subtypeOf (BUnionType BIntType BBoolType) (BUnionType BIntType (BUnionType BNoneType BBoolType))
 let testa4 = subtypeOf (BUnionType BIntType BBoolType) (BUnionType BBoolType BIntType)
-
 let testa5 = subtypeOf (BTupleType false 1 (SCons BIntType 0 SNil)) (BTupleType false 1 (SCons BIntType 0 SNil))
-
 let testa6 = subtypeOf (BTupleType false 1 (SCons BIntType 0 SNil)) (BTupleType false 1 (SCons BBoolType 0 SNil))
 let testa7 = subtypeOf (BTupleType false 2 (SCons BIntType 1 (SCons BBoolType 0 SNil))) (BTupleType false 1 (SCons BBoolType 0 SNil))
 let testa8 = subtypeOf (BTupleType false 2 (SCons BIntType 1 (SCons BBoolType 0 SNil))) (BTupleType false 2 (SCons BIntType 1 (SCons BBoolType 0 SNil)))
@@ -55,7 +52,7 @@ let testb12 = BTuple 0 SNil
 // let testb14 = isTuple 10 testb12
 
 (* Testing: getType *)
-let testc1 = BTuple 2 (SCons aaa 1 ((SCons testb0) 0 SNil))
+let testc1 = BTuple 2 (SCons test_a 1 ((SCons testb0) 0 SNil))
 let testc2 = getType testb0
 let testc3 = getType testb1
 let testc4 = getType testc1
@@ -99,12 +96,23 @@ let _ = assert (forall x y z. extractBool (greaterOrEq (maxWithUnion2 (BInt x) (
 && (extractBool ((eqTerm (maxWithUnion2 (BBool z) (BInt x)) (BInt x))))
 )
 
+(* ----------------------------------------------------------------------------------------------------------------------------------------------------------- *)
+
 val max : x:bosqueTerm{isInt x} -> y:bosqueTerm{isInt y} -> z:bosqueTerm{isInt z}
 let max x y = if (extractBool (greaterOrEq x y)) then x else y
 
 let _ = assert (forall x y. extractBool (greaterOrEq (max (BInt x) (BInt y)) (BInt x) )
 && extractBool (greaterOrEq (max (BInt x) (BInt y)) (BInt y))
 && (extractBool (eqTerm (max (BInt x) (BInt y)) (BInt x)) || extractBool (eqTerm (max (BInt x) (BInt y)) (BInt y)))
+)
+
+// New version of max using subtypeOf
+val max' : x:bosqueTerm{subtypeOf (BIntType) (getType x)} -> y:bosqueTerm{subtypeOf (BIntType) (getType y)} -> z:bosqueTerm{subtypeOf (BIntType) (getType z)}
+let max' x y = if (extractBool (greaterOrEq x y)) then x else y
+
+let _ = assert (forall x y. extractBool (greaterOrEq (max' (BInt x) (BInt y)) (BInt x) )
+&& extractBool (greaterOrEq (max' (BInt x) (BInt y)) (BInt y))
+&& (extractBool (eqTerm (max' (BInt x) (BInt y)) (BInt x)) || extractBool (eqTerm (max' (BInt x) (BInt y)) (BInt y)))
 )
 
 // // The following fails, as expected
@@ -114,6 +122,8 @@ let _ = assert (forall x y. extractBool (greaterOrEq (max (BInt x) (BInt y)) (BI
 // && (extractBool (eqTerm (max (BInt x) (BBool z)) (BInt x)))
 // )
 
+(* ----------------------------------------------------------------------------------------------------------------------------------------------------------- *)
+
 val maxWithTuple : x:bosqueTerm{isTuple false 2 (SCons (BIntType) 1 (SCons (BBoolType) 0 SNil)) x}
   -> y:bosqueTerm{isInt y} 
   -> z:bosqueTerm{isInt z}
@@ -121,134 +131,136 @@ let maxWithTuple x y =
   let xAt0 = nthTuple 0 2 x in 
     if (extractBool (greaterOrEq xAt0 y)) then xAt0 
     else y
+
+let typeTuple2BIntBBool = BTupleType false 2 (SCons (BIntType) 1 (SCons (BBoolType) 0 SNil))
+
+// New version of maxWithTuple using subtypeOf
+val maxWithTuple' : x:bosqueTerm{subtypeOf typeTuple2BIntBBool (getType x)}
+  -> y:bosqueTerm{isInt y} 
+  -> z:bosqueTerm{isInt z}
+let maxWithTuple' x y = 
+  let xAt0 = nthTuple 0 2 x in 
+    if (extractBool (greaterOrEq xAt0 y)) then xAt0 
+    else y
     
 (* Testing: maxWithTuple *)
-let test4a = maxWithTuple (testb0) (BInt 1203)
-let test4b = maxWithTuple (testb0) (BInt (-12))
+let teste0 = maxWithTuple (testb0) (BInt 1203)
+let teste1 = maxWithTuple (testb0) (BInt (-12))
+let teste0' = maxWithTuple' (testb0) (BInt 1203)
+let teste1' = maxWithTuple' (testb0) (BInt (-12))
 
 let _ = assert (forall x y . extractBool (greaterOrEq (maxWithTuple x y) (nthTuple 0 2 x)))
 
 let _ = assert (forall x y . (eqType (getType (nthTuple 0 2 x)) BIntType) ==> extractBool (greaterOrEq (maxWithTuple x y) (nthTuple 0 2 x)))
 
-val maxWithTuple2 : x:bosqueTerm{isTuple false 2 (SCons (BIntType) 1 (SCons (BBoolType) 0 SNil)) x} 
+(* ----------------------------------------------------------------------------------------------------------------------------------------------------------- *)
+
+val maxWithTuple'' : x:bosqueTerm{isTuple false 2 (SCons (BIntType) 1 (SCons (BBoolType) 0 SNil)) x} 
   -> y:bosqueTerm{isInt y} 
   -> z:bosqueTerm{isInt z}
-let maxWithTuple2 x y = match x with 
+let maxWithTuple'' x y = match x with 
 | BTuple 2 seq -> 
   let xAt0 = nthTuple 0 2 x in 
     match xAt0 with 
     | BInt x1 -> if (extractBool (greaterOrEq xAt0 y)) then xAt0 else y
     | _ -> BError
 
-val withOpenTuple : x:bosqueTerm{subtypeOf (BTupleType true 0 SNil) (getType x)} -> Tot bool
-let withOpenTuple x = match x with 
-| BTuple m seq -> false
+(* Testing: maxWithTuple'' *)
+let test5a = maxWithTuple'' (testb0) (BInt 1203)
+let test5b = maxWithTuple'' (testb0) (BInt (-12))
+
+// let _ = assert (forall x y . extractBool (greaterOrEq (maxWithTuple2 x y) (nthTuple 0 2 x)))
+
+let _ = assert (forall x y . (eqType (getType (nthTuple 0 2 x)) BIntType) ==> extractBool (greaterOrEq (maxWithTuple'' x y) (nthTuple 0 2 x)))
+
+(* ----------------------------------------------------------------------------------------------------------------------------------------------------------- *)
+
+let closedTuple2_Int_Bool = (BTupleType false 2 (SCons (BIntType) 1 (SCons (BBoolType) 0 SNil)))
+
+// New version of maxWithTuple'' using subtypeOf
+val maxWithTuple''' : x:bosqueTerm{(subtypeOf closedTuple2_Int_Bool (getType x))} 
+  -> y:bosqueTerm{isInt y} 
+  -> z:bosqueTerm{isInt z}
+let maxWithTuple''' x y = match x with 
+| BTuple 2 seq -> 
+  let xAt0 = nthTuple 0 2 x in 
+    if (extractBool (greaterOrEq xAt0 y)) then xAt0 else y
+
+// New version of maxWithTuple''' (shorter representation)
+val maxWithTuple'''' : x:bosqueTerm{(subtypeOf closedTuple2_Int_Bool (getType x))} 
+  -> y:bosqueTerm{isInt y} 
+  -> z:bosqueTerm{isInt z}
+let maxWithTuple'''' x y = let xAt0 = nthTuple 0 2 x in 
+    if (extractBool (greaterOrEq xAt0 y)) then xAt0 else y
+  
+// // Idk why the following doesn't work like maxWithTuple''''
+// val maxWithTuple''''' : x:bosqueTerm{subtypeOf (BTupleType false 2 (SCons (BIntType) 1 (SCons (BBoolType) 0 SNil))) (getType x)} 
+//   -> y:bosqueTerm{isInt y} 
+//   -> z:bosqueTerm
+// let maxWithTuple''''' x y = match x with 
+// | BTuple 2 seq -> 
+//   let xAt0 = nthTuple 0 2 x in 
+//     if (extractBool (greaterOrEq xAt0 y)) then xAt0 else y
+
+// // The following two examples are interesting because they maxWithTuple'''' fails to
+// // type check the fact that (BTuple 2 (SCons (BInt 2) 1 (SCons (BBool true) 0 SNil))) has
+// // type [BIntType, BBoolType]
+// let testh0 = let whatt = (BTuple 2 (SCons (BInt 2) 1 (SCons (BBool true) 0 SNil))) in maxWithTuple'''' whatt (BInt 33)
+// let testh1 = maxWithTuple'''' (BTuple 2 (SCons (BInt 2) 1 (SCons (BBool true) 0 SNil))) (BInt 33) 
+
+let tupleTypeExample = (BTuple 2 (SCons (BInt 2) 1 (SCons (BBool true) 0 SNil)))
+
+let testg0 = subtypeOf (BTupleType false 2 (SCons (BIntType) 1 (SCons (BBoolType) 0 SNil))) (getType tupleTypeExample)
+let testg1 = subtypeOf (BTupleType false 2 (SCons (BIntType) 1 (SCons (BBoolType) 0 SNil))) (getType (BTuple 2 (SCons (BInt 2) 1 (SCons (BBool true) 0 SNil))))
+
+// This approach `fixes` testh0 and testh1
+let testg2 = maxWithTuple'''' tupleTypeExample (BInt 33)
+
+(* ----------------------------------------------------------------------------------------------------------------------------------------------------------- *)
 
 // val withClosedTuple : x:bosqueTerm{subtypeOf (BTupleType false 2 (SCons (BIntType) 1 (SCons (BBoolType) 0 SNil))) (getType x)} -> Tot int
 // let withClosedTuple x = match x with 
 // | BTuple _ _ -> 0
 
-let closedTuple2_Int_Bool = (BTupleType false 2 (SCons (BIntType) 1 (SCons (BBoolType) 0 SNil)))
+val withOpenTuple : x:bosqueTerm{subtypeOf (BTupleType true 0 SNil) (getType x)} -> Tot bool
+let withOpenTuple x = match x with 
+| BTuple m seq -> false
 
-val maxWithTuple2'' : x:bosqueTerm{(subtypeOf closedTuple2_Int_Bool (getType x))} 
-  -> y:bosqueTerm{isInt y} 
-  -> z:bosqueTerm{isInt z}
-let maxWithTuple2'' x y = match x with 
-| BTuple 2 seq -> 
-  let xAt0 = nthTuple 0 2 x in 
-    if (extractBool (greaterOrEq xAt0 y)) then xAt0 else y
-
-val maxWithTuple2''' : x:bosqueTerm{(subtypeOf closedTuple2_Int_Bool (getType x))} 
-  -> y:bosqueTerm{isInt y} 
-  -> z:bosqueTerm{isInt z}
-let maxWithTuple2''' x y = let xAt0 = nthTuple 0 2 x in 
-    if (extractBool (greaterOrEq xAt0 y)) then xAt0 else y
-  
-// // Idk why the following doesn't work like maxWithTuple2''
-// val maxWithTuple2' : x:bosqueTerm{subtypeOf (BTupleType false 2 (SCons (BIntType) 1 (SCons (BBoolType) 0 SNil))) (getType x)} 
-//   -> y:bosqueTerm{isInt y} 
-//   -> z:bosqueTerm
-// let maxWithTuple2' x y = match x with 
-// | BTuple 2 seq -> 
-//   let xAt0 = nthTuple 0 2 x in 
-//     if (extractBool (greaterOrEq xAt0 y)) then xAt0 else y
-
-let openTuple2_Int_Bool = (BTupleType true 2 (SCons (BIntType) 1 (SCons (BBoolType) 0 SNil)))
-
-val withOpenTuple2 : x:bosqueTerm{subtypeOf openTuple2_Int_Bool (getType x)} -> Tot bool
-let withOpenTuple2 x = match x with
-| BTuple 2 seq -> false
-| BTuple 3 seq -> true
-| BTuple m seq -> true
-
-let ahhhh1 = BTuple 1 (SCons (BInt 3) 0 SNil)
-let ahhhh2 = BTuple 2 (SCons (BBool true) 1 (SCons (BInt 3) 0 SNil) )
-let ahhhh2' = BTuple 2 (SCons (BInt 0) 1 (SCons (BBool true) 0 SNil) )
-let ahhhh3 = BTuple 3 (SCons (BInt 0) 2 (SCons (BBool true) 1 (SCons (BInt 12) 0 SNil)) )
-// Demo: change the ahhhhx where x is {1, 2, 2', 3}
-let bhhhh = withOpenTuple2 ahhhh3
-
-let openTuple2_openTuple2Int_Bool_Bool = (BTupleType true 2 (SCons ((BTupleType true 2 (SCons (BIntType) 1 (SCons (BBoolType) 0 SNil)))) 1 (SCons (BBoolType) 0 SNil)))
-
-val withOpenTupleTuple2 : x:bosqueTerm{subtypeOf openTuple2_openTuple2Int_Bool_Bool (getType x)} -> Tot (bool)
-let withOpenTupleTuple2 x = match x with
-| BTuple 2 seq -> false
-| BTuple 3 seq -> true
-| BTuple m seq -> true
-
-val withOpenTupleTuple3 : x:bosqueTerm{subtypeOf openTuple2_openTuple2Int_Bool_Bool (getType x)} -> Tot (y:bosqueTerm{isInt y})
-let withOpenTupleTuple3 x = match x with
-| BTuple 2 seq -> let temp1 = nthTuple 0 2 x in let temp2 = nthTuple 0 2 temp1 in temp2
-| BTuple 3 seq -> let temp1 = nthTuple 0 2 x in let temp2 = nthTuple 0 2 temp1 in temp2
-| BTuple m seq -> let temp1 = nthTuple 0 2 x in let temp2 = nthTuple 0 2 temp1 in temp2
-
-// // Idk why the following doesn't work like withOpenTuple2'
-// val withOpenTuple2' : x:bosqueTerm{subtypeOf (BTupleType true 2 (SCons (BIntType) 1 (SCons (BBoolType) 0 SNil))) (getType x)} -> Tot bool
-// let withOpenTuple2' x = match x with
+// // Idk why the following doesn't work
+// val withOpenTuple2 : x:bosqueTerm{subtypeOf (BTupleType true 2 (SCons (BIntType) 1 (SCons (BBoolType) 0 SNil))) (getType x)} -> Tot bool
+// let withOpenTuple2 x = match x with
 // | BTuple 2 seq -> false
 // | BTuple 3 seq -> false 
 // | BTuple m seq -> true
 
+let openTuple2_Int_Bool = (BTupleType true 2 (SCons (BIntType) 1 (SCons (BBoolType) 0 SNil)))
 
+// This new version of withOpenTuple2 works! It needed the type to be declare (?!)
+val withOpenTuple2' : x:bosqueTerm{subtypeOf openTuple2_Int_Bool (getType x)} -> Tot bool
+let withOpenTuple2' x = match x with
+| BTuple 2 seq -> false
+| BTuple 3 seq -> true
+| BTuple m seq -> true
 
-let tupleTypeExample = (BTuple 2 (SCons (BInt 2) 1 (SCons (BBool true) 0 SNil)))
+let testf0 = BTuple 1 (SCons (BInt 3) 0 SNil)
+let testf1 = BTuple 2 (SCons (BBool true) 1 (SCons (BInt 3) 0 SNil) )
+let testf2 = BTuple 2 (SCons (BInt 0) 1 (SCons (BBool true) 0 SNil) )
+let testf3 = BTuple 3 (SCons (BInt 0) 2 (SCons (BBool true) 1 (SCons (BInt 12) 0 SNil)) )
+// Demo: change the testfx where x is {0, 1, 2, 3}
+let testf4 = withOpenTuple2' testf3
 
-let testing = subtypeOf (BTupleType false 2 (SCons (BIntType) 1 (SCons (BBoolType) 0 SNil))) (getType tupleTypeExample)
-let testing2 = subtypeOf (BTupleType false 2 (SCons (BIntType) 1 (SCons (BBoolType) 0 SNil))) (getType (BTuple 2 (SCons (BInt 2) 1 (SCons (BBool true) 0 SNil))))
+let openTuple2_openTuple2Int_Bool_Bool = (BTupleType true 2 (SCons ((BTupleType true 2 (SCons (BIntType) 1 (SCons (BBoolType) 0 SNil)))) 1 (SCons (BBoolType) 0 SNil)))
 
-let hmm = maxWithTuple2'' tupleTypeExample (BInt 33)
+val withOpenTupleTuple : x:bosqueTerm{subtypeOf openTuple2_openTuple2Int_Bool_Bool (getType x)} -> Tot (bool)
+let withOpenTupleTuple x = match x with
+| BTuple 2 seq -> false
+| BTuple 3 seq -> true
+| BTuple m seq -> true
 
-// let hmm2 = let whatt = (BTuple 2 (SCons (BInt 2) 1 (SCons (BBool true) 0 SNil))) in maxWithTuple2'' whatt (BInt 33)
+val withOpenTupleTuple' : x:bosqueTerm{subtypeOf openTuple2_openTuple2Int_Bool_Bool (getType x)} -> Tot (y:bosqueTerm{isInt y})
+let withOpenTupleTuple' x = match x with
+| BTuple 2 seq -> let temp1 = nthTuple 0 2 x in let temp2 = nthTuple 0 2 temp1 in temp2
+| BTuple 3 seq -> let temp1 = nthTuple 0 2 x in let temp2 = nthTuple 0 2 temp1 in temp2
+| BTuple m seq -> let temp1 = nthTuple 0 2 x in let temp2 = nthTuple 0 2 temp1 in temp2
 
-let hmm3 = maxWithTuple2'' (BTuple 2 (SCons (BInt 2) 1 (SCons (BBool true) 0 SNil))) (BInt 33)
-
-val maxWithTuple3 : x:bosqueTerm{isTuple true 2 (SCons (BIntType) 1 (SCons (BBoolType) 0 SNil)) x} 
-  -> y:bosqueTerm{isInt y} 
-  -> z:bosqueTerm
-let maxWithTuple3 x y = match x with 
-| BTuple 2 seq ->
-  let xAt0 = nthTuple 0 2 x in 
-    assert (isInt xAt0);
-    match xAt0 with 
-    | BInt x1 -> if (extractBool (greaterOrEq xAt0 y)) then xAt0 else y
-    | _ -> BError
-
-val maxWithTuple4 : x:bosqueTerm{isTuple2 false 2 (SCons (BIntType) 1 (SCons (BBoolType) 0 SNil)) x} 
-  -> y:bosqueTerm{isInt y} 
-  -> z:bosqueTerm{isInt z}
-let maxWithTuple4 x y = 
-  let xAt0 = nthTuple 0 2 x in 
-    assert (isInt xAt0);
-    match xAt0 with 
-    | BInt x1 -> if (extractBool (greaterOrEq xAt0 y)) then xAt0 else y
-    | _ -> BError
-
-(* Testing: maxWithTuple2 *)
-let test5a = maxWithTuple2 (testb0) (BInt 1203)
-let test5b = maxWithTuple2 (testb0) (BInt (-12))
-
-// let _ = assert (forall x y . extractBool (greaterOrEq (maxWithTuple2 x y) (nthTuple 0 2 x)))
-
-let _ = assert (forall x y . (eqType (getType (nthTuple 0 2 x)) BIntType) ==> extractBool (greaterOrEq (maxWithTuple2 x y) (nthTuple 0 2 x)))
-
-(* ---------------------------------------------------------------- *)
+(* ----------------------------------------------------------------------------------------------------------------------------------------------------------- *)
